\documentclass[a4paper,12pt]{article}
\usepackage[utf8]{inputenc}
\usepackage[legalpaper, margin=0.5in]{geometry}
\usepackage{amsmath}

\setlength{\parindent}{0em}
\setlength{\parskip}{1em}

\title{Week 2: Exponentials}
\author{Jinil Jang }
\date{October 2019}

\begin{document}

\maketitle

\section{Algebraic Properties}

$$e^xe^y = e^{x+y}$$
$$(e^x)^y = e^{xy}$$

\section{Differential / Integral Properties}

$$\frac{d}{dx}e^x = e^x$$
$$\int e^xdx = e^x + C$$

\section{Euler's Formula}

$$e^{ix} = cos x + i sin x$$

\section{Definition of $e^x$}

\begin{equation}
\begin{split}
e^x & = 1 + x + \frac{1}{2}x^2 + \frac{1}{6}x^3 + \frac{1}{24}x^4 + \frac{1}{120}x^5 + \cdots \\
 & = 1 + x + \frac{1}{2!}x^2 + \frac{1}{3!}x^3 + \frac{1}{4!}x^4 + \frac{1}{5!}x^5 + \cdots \\
 & = \Sigma_{k=0}^\infty \frac{x^k}{k!} 
\end{split}
\end{equation}

\section{Polynomials}
$$\frac{d}{dx}x^k = kx^{k-1}$$
$$\int x^k dx = \frac{1}{k+1}x^{k+1} + C$$

\section{Prove: Differential / Integral of $e^x$}
\begin{equation}
\begin{split}
\frac{d}{dx}e^x & = \frac{d}{dx}(1 + x + \frac{1}{2!}x^2 + \frac{1}{3!}x^3 + \frac{1}{4!}x^4 + \cdots) \\
 & = 0 + 1 + \frac{1}{2!}2x + \frac{1}{3!}3x^2 + \frac{1}{4!}4x^3 + \cdots \\
 & = 1 + x + \frac{1}{2!}x^2 + \frac{1}{3!}x^3 + \frac{1}{4!}x^4 + \cdots \\
 & = e^x
\end{split}
\end{equation}

\begin{equation}
\begin{split}
\int e^x dx & = \int (1 + x + \frac{1}{2!}x^2 + \frac{1}{3!}x^3 + \frac{1}{4!}x^4 + \cdots)dx \\
 & = x + \frac{1}{2}x^2 + \frac{1}{2!}\frac{1}{3}x^3 + \frac{1}{3!}\frac{1}{4}x^4 + \cdots + C\\
 & = e^x + C
\end{split}
\end{equation}

\section{Euler}

\begin{equation}
\begin{split}
e^{ix} & = 1 + ix + \frac{1}{2!}i^2x^2 + \frac{1}{3!}i^3x^3 + \frac{1}{4!}i^4x^4 + \frac{1}{5!}i^5x^5 + \cdots \\
 & = 1 + ix - \frac{1}{2!}x^2 - \frac{1}{3!}ix^3 + \frac{1}{4!}x^4 + \frac{1}{5!}ix^5 + \cdots \\
 & = (1 - \frac{1}{2!}x^2 + \frac{1}{4!}x^4 + \cdots) + i(x - \frac{1}{3!}x^3 + \frac{1}{5!}x^5 + \cdots) \\
 & = cos x + i sin x
\end{split}
\end{equation}

\section{Trigonometrics}

\begin{equation}
\begin{split}
cos x & = 1 - \frac{1}{2!}x^2 + \frac{1}{4!}x^4 - \frac{1}{6!}x^6 + \cdots \\
 & = \Sigma_{k=0}^\infty {(-1)}^k \frac{x^{2k}}{(2k)!}
\end{split}
\end{equation}

\begin{equation}
\begin{split}
sin x & = x - \frac{1}{3!}x^3 + \frac{1}{5!}x^5 - \frac{1}{7!}x^7 + \cdots \\
 & = \Sigma_{k=0}^\infty {(-1)}^k \frac{x^{2k+1}}{(2k+1)!}
\end{split}
\end{equation}

\begin{equation}
\begin{split}
\frac{d}{dx}sin x & = \frac{d}{dx}(x - \frac{1}{3!}x^3 + \frac{1}{5!}x^5 - \frac{1}{7!}x^7 + \cdots) \\
 & = 1 - \frac{1}{3!}3x^2 + \frac{1}{5!}5x^4 - \frac{1}{7!}7x^6 + \cdots \\
 & = 1 - \frac{1}{2!}x^2 + \frac{1}{4!}x^4 - \frac{1}{6!}x^6 + \cdots \\
 & = cos x
\end{split}
\end{equation}

\begin{equation}
\begin{split}
\frac{d}{dx}\Sigma_{k=0}^\infty (-1)^k \frac{x^{2k+1}}{(2k+1)!} = \Sigma_{k=0}^\infty {(-1)}^k \frac{x^{2k}}{(2k)!}
\end{split}
\end{equation}

\end{document}
